enter_queue and Wenum defined

FormalizationOfComputability/PhiSeq.lean
@@ -10,19 +10,19 @@ import Mathlib.Data.Set.Finite.Lattice
 import Mathlib.Data.Set.Card
 
 /- # Wₑ as a sequence
-This file builds W_seq, which enumerates the elements n of W_e
-in the order in which ϕ_e(n) halts -/
+This file builds W_seq, which enumerates the elements n of W_e in the order that each ϕ_e(n) halts -/
 
 namespace Computability
 
 open Nat
 open Nat.Partrec
 open Nat.Partrec.Code
+open List
 
 /- The elements whose computations first halt at stage s, in increasing order. By definition,
 these elements are less than s. -/
 def PhiNewList (e s : ℕ) : List ℕ :=
-  (List.range s).filter (λ n => (Phi_s_halts e s n ∧ ¬ Phi_s_halts e (s-1) n))
+  (range s).filter (λ n => (Phi_s_halts e s n ∧ ¬ Phi_s_halts e (s-1) n))
 
 def PhiNew (e s : ℕ) : Finset ℕ := (PhiNewList e s).toFinset
 
@@ -95,13 +95,6 @@ lemma PhiNew_pairwise_disjoint (e : ℕ) :
 lemma PhiNew_is_new (e s : ℕ) : (PhiNew e s) ∩ (W_s e (s-1)) = ∅ := by
   rw [PhiNew_eq_Ws_diff]
   simp
-
-/- W_{e, s+1} is exactly W_{e, s} and the new elements at stage s+1. -/
-lemma Ws_plus_one_eq (e s : ℕ) : W_s e (s+1) = (W_s e s) ∪ (PhiNew e (s+1)) := by
-    rw [PhiNew_eq_Ws_diff]
-    simp
-    apply W_s_mono e s (s+1)
-    simp
 
 /- It is sometimes useful to work with W_{e,s} instead of W_{e, s+1} -/
 lemma Ws_eq (e s : ℕ) : W_s e s = (W_s e (s-1)) ∪ (PhiNew e s) := by
@@ -225,36 +218,39 @@ lemma Union_split (t : ℕ) (p : ℕ → Set ℕ) :
     · intro i h3
       exact Set.subset_iUnion_of_subset i fun ⦃a⦄ a ↦ a
 
+
 /- TFAE :
+Eventually all PhiNew e s = ∅
 W_e is finite
-W_e = some W_{e, s}
-Eventually there are no new elements -/
-lemma PhiNew_stabilizes_implies_We_finite (e t : ℕ) (h : ∀ s > t, PhiNew e s = ∅) :
+There is an s such that W_e = W_{e, s}
+-/
+
+lemma PhiNew_stabilizes_implies_We_finite (e s : ℕ) (h : ∀ t > s, PhiNew e t = ∅) :
     (W e).Finite := by
   rw [We_eq_union_WsNew, Set.finite_iUnion_iff]
   · simp
-    apply Set.Finite.subset (Set.finite_le_nat t)
+    apply Set.Finite.subset (Set.finite_le_nat s)
     simp
-    intro s h1
+    intro t h1
     contrapose h1
     simp at h1
     simp [h, h1]
   · simp
     intro i j h1
     apply PhiNew_pairwise_disjoint
-    simp
-    simp
-    simp
-    exact h1
+    · simp
+    · simp
+    · simp
+      exact h1
 
-lemma PhiNew_stabilizes_implies_We_eq_Ws (e t : ℕ) (h : ∀ s > t, PhiNew e s = ∅) :
-    W e = W_s e t := by
+lemma PhiNew_stabilizes_implies_We_eq_Ws (e s : ℕ) (h : ∀ t > s, PhiNew e t = ∅) :
+    W e = W_s e s := by
   rw [We_eq_union_WsNew]
   apply subset_antisymm
   · intro x h1
     simp at h1
     obtain ⟨r, h1⟩ := h1
-    have h2 : r ≤ t := by
+    have h2 : r ≤ s := by
       contrapose h1
       simp at h1
       apply h at h1
@@ -273,8 +269,8 @@ lemma PhiNew_stabilizes_implies_We_eq_Ws (e t : ℕ) (h : ∀ s > t, PhiNew e s 
     simp
     use r
 
-lemma We_finite_implies_Ws_stabilizes (e : ℕ) (h : (W e).Finite) :
-    ∃ t, ∀ s > t, PhiNew e s = ∅ := by
+lemma We_finite_implies_PhiNew_stabilizes (e : ℕ) (h : (W e).Finite) :
+    ∃ s, ∀ t > s, PhiNew e t = ∅ := by
   rw [We_eq_union_WsNew, Set.finite_iUnion_iff] at h
   simp at h
   have h1 :  ∃ P : Finset ℕ, ∀ n, n ∈ P ↔ n ∈ {i | (PhiNew e i).Nonempty} := by
@@ -306,17 +302,17 @@ lemma We_finite_implies_Ws_stabilizes (e : ℕ) (h : (W e).Finite) :
     simp
     exact h1
 
-lemma We_finite_iff_Ws_stabilizes (e : ℕ) :
+lemma We_finite_iff_PhiNew_stabilizes (e : ℕ) :
     (W e).Finite ↔ (∃ t, ∀ s > t, PhiNew e s = ∅) := by
   constructor
-  · apply We_finite_implies_Ws_stabilizes e
+  · apply We_finite_implies_PhiNew_stabilizes e
   · intro ⟨t, h⟩
     apply PhiNew_stabilizes_implies_We_finite
     exact h
 
 lemma We_finite_iff_We_eq_Ws (e : ℕ) : (W e).Finite ↔ ∃ s, W e = W_s e s := by
   constructor
-  · rw [We_finite_iff_Ws_stabilizes]
+  · rw [We_finite_iff_PhiNew_stabilizes]
     intro ⟨t, h⟩
     use t
     apply PhiNew_stabilizes_implies_We_eq_Ws
@@ -332,44 +328,34 @@ lemma PhiNew_runtime (y e s : ℕ) : y ∈ PhiNew e s ↔ s ∈ runtime e y := b
   · simp [PhiNew, PhiNewList, W_s]
     intro h h1 h2
     constructor
-    · constructor
-      · exact Option.isSome_iff_exists.mpr h1
-      · intro m hm
-        have h3 : Phi_s_halts e s y → y < s := by
-          apply halt_input_bound
-        apply phi_halts_mono_reverse e m at h2
-        · unfold Phi_s_diverges Phi_s_halts at h2
-          push_neg at h2
-          exact Option.eq_none_iff_forall_ne_some.mpr h2
-        · exact le_sub_one_of_lt hm
-    exact Option.isSome_iff_exists.mpr h1
-  · intro ⟨⟨h, h1⟩, h2⟩
+    · exact Option.isSome_iff_exists.mpr h1
+    · intro m hm
+      have h3 : Phi_s_halts e s y → y < s := by
+        apply halt_input_bound
+      apply phi_halts_mono_reverse e m at h2
+      · unfold Phi_s_diverges Phi_s_halts at h2
+        push_neg at h2
+        exact Option.eq_none_iff_forall_ne_some.mpr h2
+      · exact le_sub_one_of_lt hm
+  · intro ⟨h, h1⟩
     apply Option.isSome_iff_exists.mp at h
     simp [PhiNew, PhiNewList]
     constructor
     · apply halt_input_bound e
-      unfold Phi_s_halts
-      exact h
+      simp [Phi_s_halts, h]
     · constructor
       · exact h
       · unfold Phi_s_halts
         push_neg
         intro y
         by_cases h2 : s=0
-        · simp [h2]
-          unfold Phi_s
-          simp
-        · have h3 : s - 1 < s := by
-            exact sub_one_lt h2
-          apply h1 at h3
-          simp [h3]
+        · simp [h2, Phi_s]
+        · simp [h1, sub_one_lt, h2]
 
 /- The elements in W_e enumerated up to stage s, in the order they appeared -/
 def WPrefix (e : ℕ) : ℕ → List ℕ
 | 0     => []
 | s + 1 => (WPrefix e s) ++ (PhiNewList e (s+1))
-
-open List.Nodup
 
 /- WPrefix e s is exactly W_{e, s} in order of enumeration -/
 lemma Ws_eq_prefix (e s : ℕ) : W_s e s = (WPrefix e s).toFinset := by
@@ -380,7 +366,7 @@ lemma Ws_eq_prefix (e s : ℕ) : W_s e s = (WPrefix e s).toFinset := by
     simp [WPrefix]
     by_cases h1 : y ∈ (W_s e s)
     · left
-      rw [← List.mem_toFinset, ← hs]
+      rw [← mem_toFinset, ← hs]
       exact h1
     · right
       simp [PhiNew, PhiNewList]
@@ -395,7 +381,7 @@ lemma Ws_eq_prefix (e s : ℕ) : W_s e s = (WPrefix e s).toFinset := by
           tauto
     · intro x h
       simp [WPrefix, PhiNew, W_s] at h
-      rw [PhiNewList_mem, ← List.mem_toFinset, ← hs] at h
+      rw [PhiNewList_mem, ← mem_toFinset, ← hs] at h
       simp [W_s]
       simp [W_s] at h
       rcases h with h | h
@@ -411,10 +397,18 @@ lemma Ws_eq_prefix (e s : ℕ) : W_s e s = (WPrefix e s).toFinset := by
         · exact h.left.right
 
 lemma WPrefix_mem (e s n : ℕ) : n ∈ WPrefix e s ↔ n ∈ W_s e s := by
-  rw [← List.mem_toFinset, Ws_eq_prefix]
+  rw [← mem_toFinset, Ws_eq_prefix]
+
+lemma WPrefix_phi (e n : ℕ) : (∃ s, n ∈ WPrefix e s) ↔ Phi_halts e n := by
+  rw [phi_halts_stage_exists, exists_congr]
+  intro a
+  rw [← W_s_Phi_s]
+  exact WPrefix_mem e a n
+
+open List.Nodup
 
 /- Elements cannot be enumerated twice-/
-lemma nodup_WPrefix (e s : ℕ) : List.Nodup (WPrefix e s) := by
+lemma nodup_WPrefix (e s : ℕ) : Nodup (WPrefix e s) := by
   induction' s with s ih
   · unfold WPrefix
     simp
@@ -422,7 +416,7 @@ lemma nodup_WPrefix (e s : ℕ) : List.Nodup (WPrefix e s) := by
     apply append
     · exact ih
     · apply List.Nodup.filter
-      exact List.nodup_range
+      exact nodup_range
     · unfold List.Disjoint
       intro a h h1
       simp [PhiNewList_mem, PhiNew_eq_Ws_diff, Ws_eq_prefix] at h1
@@ -443,43 +437,197 @@ lemma WPrefix_mono (e s t : ℕ) (h : s ≤ t) :
       apply List.IsPrefix.trans h2
       simp [WPrefix]
 
+theorem idxOf?_mem {α : Type} [inst : DecidableEq α] {a : α} {n : ℕ} {L : List α}
+    (h : n = List.idxOf? a L) : L[n]? = a := by
+  have := List.of_findIdx?_eq_some h.symm
+  generalize hi : L[n]? = i at this ⊢
+  cases i <;> simp_all
 
-/- The first n elements of W_e, in enumeration order (if it has that many)-/
-/- partial def WnUpToAux (e n s : ℕ) (acc : List ℕ) : Option (List ℕ) :=
-  if acc.length ≥ n then
-    some acc
-  else
-    WnUpToAux e n (s + 1) (acc ++ ((WPrefix e s).filter (· ∉ acc)))
+theorem mem_idxOf? {α : Type} [inst : DecidableEq α] {a : α} {n : ℕ} {L : List α}
+    (h : List.Nodup L) (h1 : L[n]? = a) : n = List.idxOf? a L := by
+  have h2 : n < L.length := by
+    exact (isSome_getElem? L n).mp (Option.isSome_of_mem h1)
+  have h3 : L[n] = a := by
+    exact (List.getElem_eq_iff h2).mpr h1
+  rw [List.idxOf?, eq_comm, List.findIdx?_eq_some_iff_findIdx_eq, List.findIdx_eq]
+  constructor
+  · exact h2
+  · constructor
+    · simp [h3]
+    · intro j hjn
+      simp [← h3]
+      rw [List.Nodup.getElem_inj_iff]
+      · apply Nat.ne_of_lt hjn
+      · exact h
+  · exact h2
 
-def WnUpTo (e n : ℕ) : Option (List ℕ) :=
-  WnUpToAux e n 0 [] -/
+/- It is often useful to view elements entering one at a time, so there may be a queue
+of elements waiting to enter. This represents the elements still waiting *at* stage s,
+i.e. the head of this list will be enumerated at stage s. -/
+def enter_queue (e : ℕ) : ℕ → List ℕ
+  | 0 => []
+  | s + 1 => (enter_queue e s).tail ++ (PhiNewList e (s+1))
 
-open Stream'
-open Stream'.Seq
+/- If n is in an queue at stage s, then ϕ_{e, s}(n)↓ -/
+lemma enter_queue_halts (e s n: ℕ) (h : n ∈ enter_queue e s) : Phi_s_halts e s n := by
+  induction' s with s ih
+  · tauto
+  · unfold enter_queue at h
+    rw [List.mem_append] at h
+    cases' h with h h
+    · apply List.mem_of_mem_tail at h
+      apply ih at h
+      exact phi_halts_mono e s (s+1) n (Nat.le_add_right s 1) h
+    · simp [PhiNewList] at h
+      exact h.right.left
 
--- due to Mario Carneiro
-def PrefixUnionStage : (ℕ → List ℕ) → WSeq ℕ :=
-  Seq.corec fun f =>
-    match f 0 with
-    | [] => some (Option.none, fun n => f (n+1))
-    | .cons a _ => some (some a, fun n => (f n).tail)
+/- Elements of the queues are exactly the elements that halt -/
+lemma enter_queue_mem (e n : ℕ) : (∃ s, n ∈ enter_queue e s) ↔ Phi_halts e n := by
+  constructor
+  · intro ⟨s, h⟩
+    apply enter_queue_halts at h
+    apply (phi_halts_stage_exists e n).mpr
+    use s
+  · intro h
+    simp [phi_halts_runtime_exists, ← PhiNew_runtime_iff] at h
+    obtain ⟨r, h⟩ := h
+    use r
+    unfold enter_queue
+    cases' r with r
+    · tauto
+    · simp
+      right
+      simp [PhiNewList_mem, h]
 
-/- This tracks what happens at each stage, emitting 'none' when no elements halt-/
-def Wenum (e : ℕ) : WSeq ℕ := PrefixUnionStage (WPrefix e)
+/- The queue at stage s is a suffix of WPrefix e s.
+This is mostly here to make the next lemma easy -/
+lemma enter_queue_WPrefix (e s : ℕ) :
+    IsSuffix (enter_queue e s) (WPrefix e s) := by
+  induction' s with s ih
+  · simp [enter_queue]
+  · unfold enter_queue WPrefix
+    have h1 : (enter_queue e s).tail <:+ WPrefix e s := by
+      apply List.IsSuffix.trans (tail_suffix (enter_queue e s)) ih
+    cases' L : (enter_queue e s) with a T
+    · simp
+    · simp [L, IsSuffix] at h1
+      obtain ⟨S, h1⟩ := h1
+      use S
+      simp [← h1]
+
+/- The queues have no duplicates. -/
+lemma enter_queue_nodup (e s : ℕ) : Nodup (enter_queue e s) := by
+  have ⟨L, h⟩ := enter_queue_WPrefix e s
+  have h1 := nodup_WPrefix e s
+  rw [← h] at h1
+  exact List.Nodup.of_append_right h1
+
+/- If n is not the head of an queue, then at the next step its index decreases by 1. -/
+lemma enter_queue_dec (e n s : ℕ)
+    (h : n ∈ (enter_queue e s).tail) :
+    List.idxOf n (enter_queue e (s+1)) = List.idxOf n (enter_queue e s) - 1 := by
+  dsimp [enter_queue]
+  simp [List.idxOf_append, h]
+  cases' L : enter_queue e s with a T
+  · tauto
+  · simp [L] at h
+    apply Nat.eq_sub_of_add_eq
+    apply Eq.symm (List.idxOf_cons_ne T ?_)
+    have h2 := enter_queue_nodup e s
+    rw [L] at h2
+    apply List.Nodup.notMem at h2
+    exact Ne.symm (ne_of_mem_of_not_mem h h2)
+
+/- If PhiNew stabilizes, then eventually the queue depletes. Indeed iff is true,
+but not proved here. -/
+
+lemma queue_depletes (e s : ℕ) (h : ∀ t > s, PhiNew e t = ∅) :
+    ∃ s₁, ∀ t > s₁, enter_queue e t = [] := by
+  sorry
+  /- let l := (enter_queue e t).length
+    use t+l-1
+    intro s h1
+    simp [Wenum, new_element]
+    unfold enter_queue
+    have h2 := enter_queue_WPrefix e s
+    sorry -- can't use t - there may be a queue to be emptied -/
+
+/- The element that has been emitted at stage s, if it exists -/
+def new_element (e s : ℕ) : Option ℕ := (enter_queue e s).head?
+
+def Wenum (e : ℕ) : Stream' (Option ℕ) := new_element e
+
+lemma Wenum_finite_iff (e : ℕ) : (W e).Finite ↔ ∃ s, ∀ t > s, Wenum e t = Option.none := by
+  rw [We_finite_iff_PhiNew_stabilizes]
+  constructor
+  · intro ⟨s, h⟩
+    have ⟨s₁, h1⟩ := queue_depletes e s h
+    use s₁
+    intro t ht
+    simp [Wenum, new_element]
+    apply h1
+    exact ht
+  · intro ⟨t, h⟩
+    use t
+    intro s h1
+    simp [Wenum, new_element] at h
+    have h2 : enter_queue e s = [] := by
+      apply h
+      linarith
+    unfold enter_queue at h2
+    cases' s with s
+    · tauto
+    · simp at h2
+      ext x
+      rw [← PhiNewList_mem]
+      simp [h2]
 
 
-lemma Wenum_mem (e n x: ℕ) (h : WSeq.get? (Wenum e) n = some x) : ∃ s, x ∈ WPrefix e s := by
-  simp [Wenum, PrefixUnionStage] at h
-  induction' n with n ih
-  · simp [WSeq.get?] at h
-    cases' WPrefix e 0 with a tail!
+lemma Phi_halts_new_element (e n : ℕ) : Phi_halts e n ↔ ∃ s, new_element e s = n := by
+  simp [new_element]
+  rw [← enter_queue_mem]
+  constructor
+  · intro ⟨s, h⟩
+    have h1 : ∃ k, k = (enter_queue e s).findIdx (· = n) := by
+      exact exists_apply_eq_apply (fun a ↦ a) (idxOf n (enter_queue e s))
+    obtain ⟨k, h1⟩ := h1
+    use s+k
+    induction' k with k' ih
+    · sorry
+    · sorry
+  · intro ⟨s, h⟩
+    use s
+    exact List.mem_of_mem_head? h
 
 
-  · sorry
 
-/- def WEnum (e : ℕ) : Stream'.Seq ℕ :=
-  ⟨WStream e 1 [], by sorry
-  ⟩ -/
+
+
+
+/- ϕ_e(n) halts iff n appears in some WPrefix as the kth element -/
+lemma kth_mem (e n : ℕ) : (Phi_halts e n) ↔
+    ∃ s, (∃ k, k.isSome ∧ k = (WPrefix e s).idxOf? n) := by
+  constructor
+  · rw [phi_halts_runtime_exists]
+    intro h
+    obtain ⟨r, h⟩ := h
+    use r
+    rw [← PhiNew_runtime] at h
+    have h1 : n ∈ W_s e r := by
+      rw [Ws_eq]
+      exact Finset.mem_union_right (W_s e (r - 1)) h
+    rw [← WPrefix_mem] at h1
+    let m := (WPrefix e r).idxOf? n
+    use m
+    constructor
+    · exact List.isSome_idxOf?.mpr h1
+    · rfl
+  · intro ⟨s, ⟨k, ⟨h, h1⟩⟩⟩
+    simp [h1] at h
+    rw [← WPrefix_phi]
+    use s
+
+
 
 
 
@@ -498,7 +646,7 @@ lemma inf_inc_sigma01_seq_is_delta01 (e : ℕ) (h1 : (W e).Infinite)
 -- bounded quantifiers are decidable
 
 /- lemma sigma01_has_delta01_subset (X : Set ℕ) (hX : Sigma01 X) (hInf : X.Infinite):
-∃ (Y : Set ℕ), Delta01 Y ∧ Y.Infinite ∧ Y ⊆ X ∧ (X\Y).Infinite := by
+∃ (Y : Set ℕ), Delta01 Y ∧ Y.Infinite ∧ Y ⊆ X := by
 obtain ⟨f, ⟨hfPart, hfDom⟩⟩ := hX
 let g := f.map (fun _ => 1)
 have hfg : ∀ (x:ℕ), (f x) = some () ↔ (g x) = 1 := by
